venom/defs/venomStateScript.sml
@@ -130,7 +130,8 @@ Datatype:
     vs_code : byte list;             (* Own bytecode (CODECOPY/EXTCODECOPY) *)
     vs_params : bytes32 list;        (* Function parameters (read by PARAM) *)
     vs_ext_call_oracle :
-      evm_accounts -> address -> num -> byte list -> bool -> ext_call_result
+      evm_accounts -> address -> num -> byte list -> bool -> ext_call_result;
+    vs_allocas : (num, num # num) fmap  (* alloca_id -> (offset, size) *)
   |>
 End
 
@@ -194,7 +195,8 @@ Definition init_venom_state_def:
       <| ecr_output := 0w;
          ecr_returndata := [];
          ecr_accounts := accts;
-         ecr_new_logs := [] |>)
+         ecr_new_logs := [] |>);
+    vs_allocas := FEMPTY
   |>
 End
 
